theories/interop/wrapper_wp_boundary_laws.v
@@ -1,0 +1,136 @@
+From Coq Require Import ssreflect.
+From stdpp Require Import strings gmap.
+From melocoton Require Import named_props.
+From melocoton.mlanguage Require Import mlanguage.
+From melocoton.language Require Import language weakestpre.
+From melocoton.mlanguage Require Import weakestpre.
+From melocoton.interop Require Import wrappersem wrapperstate.
+From iris.base_logic.lib Require Import ghost_map ghost_var.
+From iris.proofmode Require Import proofmode.
+From melocoton.c_toy_lang Require Import lang melocoton.lang_instantiation melocoton.primitive_laws.
+From melocoton.ml_toy_lang Require Import lang melocoton.lang_instantiation melocoton.primitive_laws.
+From melocoton.interop Require Import linking_wp basics basics_resources wrapper_wp
+  wrapper_wp_block_sim wrapper_wp_utils.
+Import Wrap.
+
+(* lemmas to switch between the ML<->C state interp at a boundary *)
+
+Section BoundaryLaws.
+
+Context {hlc : has_lc}.
+Context {Σ : gFunctors}.
+Context `{!heapGS_ML Σ, !heapGS_C Σ}.
+Context `{!invGS_gen hlc Σ}.
+Context `{!wrapperGS Σ}.
+
+Notation MLval := ML_lang.val.
+Notation Cval := C_lang.val.
+
+Lemma wrap_interp_c_to_ml w ρc mem θ v lv (X : val → wrapstateML → store → Prop) :
+  repr_lval θ lv w →
+  c_to_ml w ρc mem X →
+  wrap_state_interp (Wrap.CState ρc mem) -∗
+  GC θ -∗
+  not_at_boundary -∗
+  block_sim v lv
+  ==∗
+  ∃ ρml σ,
+  ⌜X v ρml σ⌝ ∗
+  wrap_state_interp (Wrap.MLState ρml σ) ∗
+  at_boundary _.
+Proof.
+  iIntros (Hlv Hc_to_ml) "Hσ HGC Hnb #Hblk".
+  iNamed "Hσ". iNamed "SIC". iNamed "HGC". simplify_eq.
+
+  iAssert (⌜is_val χvirt (ζσ ∪ ζrest) v lv⌝)%I as "%Hval".
+  by iApply (block_sim_to_ghost_state with "HAχvirt HAζrest [] [] [] [] Hblk").
+  iAssert (⌜∀ k lv, roots_m !! k = Some lv → ∃ w, mem !! k = Some (Storing w) ∧ repr_lval θ lv w⌝)%I as "%Hroots".
+  1: { iIntros (kk vv Hroots).
+       iPoseProof (big_sepM_lookup with "Hrootspto") as "(%wr & Hwr & %Hw2)"; first done.
+       iExists wr. iSplit; last done. iApply (gen_heap_valid with "HσC Hwr"). }
+  apply map_Forall_lookup_2 in Hroots.
+  iPoseProof (ghost_var_agree with "HAGCθ HAθ") as "%Hagree1"; subst θ.
+  iPoseProof (ghost_var_agree with "HArootss HAroots") as "%Hagree2".
+  iMod (ghost_var_update_halves with "Hnb [HAGCbound HAbound]") as "(Hb & Hbound)".
+  (* Coq fails to infer ghost_var_fractional in time *)
+  1: iPoseProof (@fractional.fractional_merge _ _ _ _ _ _ (ghost_var_fractional _ _) with "HAGCbound HAbound") as "HH".
+  1: by assert ((1 / 4 + 1 / 4 = 1 / 2)%Qp) as -> by compute_done.
+  destruct (make_repr (θC ρc) roots_m mem) as [privmem Hpriv]; try done.
+  iMod (ghost_var_update_halves with "HAGCθ HAθ") as "(HAGCθ & HAθ)".
+  iMod (set_to_none with "HσC Hrootspto") as "(HσC & Hrootspto)"; first done.
+
+  iModIntro. iExists _, _. iSplit.
+  { iPureIntro. eapply (Hc_to_ml σMLvirt _ _ (ζσ ∪ ζrest) ζσ χvirt ζrest roots_m privmem).
+    all: try done. by rewrite map_union_comm. }
+  iSplitR "Hbound"; last by iFrame "Hbound".
+  rewrite /= /named.
+  iSplitL "HAσMLv HAnMLv HAσdom".
+  { iExists nMLv; iFrame. }
+  unfold private_state_interp, ML_state_interp, GC_token_remnant, named; cbn.
+  iFrame. iSplitL "HnC"; first by iExists _.
+  rewrite <- Hagree2.
+  iFrame "HAroots".
+  iPureIntro; split_and!.
+  1: destruct Hχvirt as (_ & HHH); apply HHH.
+  1: apply Hother_blocks.
+  1: destruct Hpriv as (mem_r & ->%repr_roots_dom & Hpriv2 & Hpriv3); by apply map_disjoint_dom.
+Qed.
+
+Lemma wrap_interp_ml_to_c vs ρml σ ws ρc mem :
+  ml_to_c vs ρml σ ws ρc mem →
+  wrap_state_interp (Wrap.MLState ρml σ) -∗
+  at_boundary wrap_lang
+  ==∗
+  wrap_state_interp (Wrap.CState ρc mem) ∗
+  not_at_boundary ∗
+  GC (θC ρc) ∗
+  (∃ lvs, block_sim_arr vs lvs ∗ ⌜Forall2 (repr_lval (θC ρc)) lvs ws⌝).
+Proof.
+  iIntros (Hml_to_c) "Hst Hb".
+  iNamed "Hst". iNamed "SIML". iNamed "HAGCrem".
+  destruct Hml_to_c as (ζσ & ζnewimm & lvs & HH).
+  destruct HH as (Hmono & Hblocks & Hprivblocks & HζC & Hζdisj &
+                    Hstore & Hvals & ? & ? & ? & Hroots & ?).
+
+  iMod (ghost_var_update_halves with "Hb HAbound") as "(Hnb & Hnb2)".
+  1: iPoseProof (@fractional.fractional _ _ (ghost_var_fractional _ _)) as "[HH _]".
+  iDestruct ("HH" with "[Hnb2]") as "(HAGCbound & HAbound)".
+  1: by assert ((1 / 4 + 1 / 4 = 1 / 2)%Qp) as <- by compute_done.
+  iClear "HH".
+  iMod (ghost_var_update_halves with "HAθ HAGCθ") as "(HAθ & HAGCθ)".
+  apply map_disjoint_union_r in Hζdisj as [Hζdisj1 Hζdisj2].
+  iMod (lstore_own_insert_many with "HAζrest") as "(HAζrest & Hζnewimm)"; first done.
+  iMod (lloc_own_mono with "HAχ") as "HAχ"; first done.
+  assert (ζσ ##ₘ ζnewimm) as Hdisj2 by by eapply is_store_blocks_is_private_blocks_disjoint.
+  assert (ζC ρc = ζσ ∪ (ζML ρml ∪ ζnewimm)) as H6B.
+  1: { rewrite map_union_assoc. rewrite (map_union_comm ζσ); first done. by symmetry. }
+  iPoseProof (block_sim_arr_of_ghost_state _ _ _ _ _ vs lvs with "HAχ HAζrest [] [] [] [] []") as "#Hsim".
+  1-5: iPureIntro. 5: eassumption. 1-3:done. 1: by apply map_disjoint_union_r.
+  iMod (set_to_some with "HAσCv Hrootspto") as "(HAσCv & Hrootspto)"; first done.
+
+  iModIntro. iFrame "Hnb". rewrite /= /named.
+  iSplitR "HAGCθ HAGCbound HArootsm HArootss Hrootspto".
+  { iSplitL "HAσCv HAnCv". { iExists nCv. iFrame. }
+    rewrite /C_state_interp /= /named.
+    iExists (ζC ρc), ζσ, (ζML ρml ∪ ζnewimm), (χC ρc), σ. iFrame.
+    rewrite Hroots. iFrame "HAroots".
+    iSplitL "HvML"; first by iExists _.
+    rewrite pub_locs_in_lstore_insert_priv_store; last done.
+    erewrite pub_locs_in_lstore_mono at 1; [| eauto..]; [].
+    iFrame "HAχNone".
+    iPureIntro. split_and!; eauto.
+    { reflexivity. }
+    { by apply map_disjoint_union_r. }
+    { rewrite dom_union_L. apply union_least.
+      - etransitivity; [ eapply Hother_blocks |].
+        eapply subseteq_dom, Hmono.
+      - eapply elem_of_subseteq. intros γ Hγ.
+        by eapply elem_of_dom_2, Hprivblocks. }
+    { split; first done. split; first apply Hmono.
+      intros γ v1 v2 HH1 HH2. simplify_map_eq. econstructor. } }
+  { iSplitL; last by (iExists _; iFrame "Hsim").
+    rewrite /GC /named. iExists (dom (rootsML ρml)), (rootsML ρml).
+    iFrame. done. }
+Qed.
+
+End BoundaryLaws.
