theories/interop/wrapper_wp_simulation.v
@@ -5,13 +5,12 @@ From melocoton.mlanguage Require Import mlanguage.
 From melocoton.language Require Import language weakestpre.
 From melocoton.mlanguage Require Import weakestpre.
 From melocoton.interop Require Import wrappersem basics_resources wrapperstate.
-From iris.base_logic.lib Require Import ghost_map ghost_var gset_bij.
-From iris.algebra Require Import gset gset_bij.
-From melocoton Require Import big_sepM_limited.
+From iris.base_logic.lib Require Import ghost_map ghost_var.
 From iris.proofmode Require Import proofmode.
 From melocoton.c_toy_lang Require Import lang melocoton.lang_instantiation melocoton.primitive_laws.
 From melocoton.ml_toy_lang Require Import lang melocoton.lang_instantiation melocoton.primitive_laws.
-From melocoton.interop Require Import linking_wp basics wrapper_wp wrapper_wp_block_sim wrapper_wp_utils wrapper_wp_ext_call_laws.
+From melocoton.interop Require Import linking_wp basics wrapper_wp wrapper_wp_block_sim
+  wrapper_wp_utils wrapper_wp_ext_call_laws wrapper_wp_boundary_laws.
 Import Wrap.
 
 Section Simulation.
@@ -46,9 +45,10 @@ Proof.
   rewrite weakestpre.wp_unfold. rewrite /weakestpre.wp_pre.
   iIntros "%σ Hσ".
   iDestruct (GC_in_C with "Hσ HGC") as "%H"; destruct H as (ρc & mem & ->).
-  iNamed "Hσ". iNamed "HGC". iNamed "SIC".
   iModIntro. iRight. iRight. iSplit.
-  1: iPureIntro; cbn; exists (fun _ => True); eexists (), _; repeat split; by eapply RetS.
+  { iPureIntro. cbn. exists (λ _, True); eexists (), _; repeat split.
+    eapply RetS; eauto using c_to_ml_True. }
+
   cbn. iIntros (X Hstep).
   destruct Hstep as ([] & e1 & Heq & Hstep).
   cbv in Heq; subst e1.
@@ -58,43 +58,13 @@ Proof.
        destruct (language.fill_class' K ec) as [?|[vv ?]];
        [exists (ExprVal a); cbn; by rewrite H
        |subst K; cbn in *; subst ec; cbn in Heq; congruence| congruence].
-  cbn in H3; injection H3; intros <-.
-  cbv in H1. subst mem0 ρc0 X0.
+  cbv [fill Wrap.fill wrap_lang] in *.
+  cbn [C_lang.to_val] in *; simplify_eq.
 
-  iAssert (⌜is_val χvirt ζfreeze v l⌝)%I as "%Hval".
-  1: iApply (block_sim_to_ghost_state with "HAχvirt HAζrest"); done.
-  iAssert (⌜∀ k v, roots_m !! k = Some v → ∃ w, mem !! k = Some (Storing w) ∧ repr_lval θ v w⌝)%I as "%Hroots".
-  1: { iIntros (kk vv Hroots). iPoseProof (big_sepM_lookup with "Hrootspto") as "(%w & Hw & %Hw2)"; first done.
-       iExists w. iSplit; last done. iApply (gen_heap_valid with "HσC Hw"). }
-  apply map_Forall_lookup_2 in Hroots.
-  iPoseProof (ghost_var_agree with "HAGCθ HAθ") as "%Hagree1"; subst θ.
-  iPoseProof (ghost_var_agree with "HArootss HAroots") as "%Hagree2"; subst roots_s.
-  iMod (ghost_var_update_halves with "Hnb [HAGCbound HAbound]") as "(Hnb & Hbound)".
-  (* Coq fails to infer ghost_var_fractional in time *)
-  1: iPoseProof (@fractional.fractional_merge _ _ _ _ _ _ (ghost_var_fractional _ _) with "HAGCbound HAbound") as "HH".
-  1: by assert ((1 / 4 + 1 / 4 = 1 / 2)%Qp) as -> by compute_done.
-  destruct (make_repr (θC ρc) roots_m mem) as [privmem Hpriv]; try done.
-  iMod (ghost_var_update_halves with "HAGCθ HAθ") as "(HAGCθ & HAθ)".
-  iMod (set_to_none with "HσC Hrootspto") as "(HσC & Hrootspto)".
-  1: done.
-
-  do 3 iModIntro. do 2 iExists _.  iSplit.
-  1: iPureIntro; eapply (H4 σMLvirt l v ζfreeze ζσ χvirt ζrest roots_m privmem).
-  all: try done.
-  1: rewrite map_union_comm; done.
-
-  iSplitR "Hv Hnb"; last first.
-  1: { iApply weakestpre.wp_value'. iFrame. }
-  cbn. iSplitL "HAσMLv HAnMLv HAσdom".
-  1: iExists nMLv; iFrame.
-  unfold private_state_interp, ML_state_interp, GC_token_remnant, named; cbn.
-  iFrame. iSplitL "HnC"; first by iExists _.
-  rewrite <- Hagree2.
-  iFrame "HAroots".
-  iPureIntro; split_and!.
-  1: destruct Hχvirt as (_ & HHH); apply HHH.
-  1: apply Hother_blocks.
-  1: destruct Hpriv as (mem_r & ->%repr_roots_dom & Hpriv2 & Hpriv3); by apply map_disjoint_dom.
+  iMod (wrap_interp_c_to_ml with "Hσ HGC Hnb [$]") as "(%ρml & %σ & HH)"; [done..|].
+  iDestruct "HH" as "(%HX & SI & Hb)".
+  do 3 iModIntro. do 2 iExists _. iSplit; first done. iFrame "SI".
+  iApply weakestpre.wp_value'. iFrame.
 Qed.
 
 Lemma wp_simulates E T ec Φ: 
@@ -162,14 +132,27 @@ Proof.
       iPureIntro; split_and!; done.
 Qed.
 
+(* TODO move? *)
+Lemma interp_ML_discarded_locs_pub ρml σ :
+  wrap_state_interp (Wrap.MLState ρml σ) -∗
+  ⌜map_Forall (λ (_ : nat) (ℓ : loc), σ !! ℓ = Some None) (pub_locs_in_lstore (χML ρml) (ζML ρml))⌝.
+Proof.
+  iNamed 1. iNamed "SIML". iRevert "HσML HAχNone". iClear "∗".
+  generalize (pub_locs_in_lstore (χML ρml) (ζML ρml)) as mm. intros mm. iStopProof.
+  induction mm as [|k l mm Hin IH] using map_ind.
+  - iIntros "_ _ _". iPureIntro. apply map_Forall_empty.
+  - iIntros "_ HL HK".
+    iDestruct (big_sepM_insert with "HK") as "[? ?]"; first done.
+    iDestruct (IH with "[$] [$] [$]") as %HIH.
+    iPoseProof (gen_heap_valid with "[$] [$]") as "%Hv".
+    iPureIntro. by apply map_Forall_insert.
+Qed.
 
-
-
-Lemma run_function_correct F (vv : list ML_lang.val) T E Φ: 
+Lemma run_function_correct F (vv : list ML_lang.val) T E Φ:
     ⌜arity F = length vv⌝
  -∗ at_boundary _
- -∗ (∀ θ ll aa ec, 
-       GC θ 
+ -∗ (∀ θ ll aa ec,
+       GC θ
     -∗ ⌜C_lang.apply_function F aa = Some ec⌝
     -∗ ⌜Forall2 (repr_lval θ) ll aa⌝
     -∗ block_sim_arr vv ll
@@ -182,140 +165,24 @@ Proof.
   unfold at_boundary; cbn. destruct σ as [ρml σ | ? ?].
   2: {iExFalso. iNamed "Hσ"; iNamed "SIC". iPoseProof (ghost_var_agree with "Hb HAbound") as "%Heq". congruence. }
   iModIntro. iRight. iRight.
-  iNamed "Hσ". iNamed "SIML". iNamed "HAGCrem".
-
-  iAssert (⌜map_Forall (λ (_ : nat) (ℓ : loc), σ !! ℓ = Some None) (pub_locs_in_lstore (χML ρml) (ζML ρml))⌝)%I with "[HσML HAχNone]" as "%Hpublocs".
-  1: { generalize (pub_locs_in_lstore (χML ρml) (ζML ρml)) as mm. intros mm. iStopProof.
-       induction mm as [|k l mm Hin IH] using map_ind; iIntros "(HH & HK)".
-       - iPureIntro. apply map_Forall_empty.
-       - iPoseProof (big_sepM_insert) as "[HL _]". 1: apply Hin.
-         iPoseProof ("HL" with "HK") as "[H1 H2]".
-         iPoseProof (IH with "[HH H2]") as "%HIH". 1: iFrame.
-         iPoseProof (gen_heap_valid with "HH H1") as "%Hv".
-         iPureIntro. apply map_Forall_insert. 1: done. split; done. }
-
-  iSplitR.
-  + iPureIntro. exists (fun _ => True). eapply mlanguage.head_prim_step. cbn.
-
-    destruct (deserialize_ML_heap_extra (ζML ρml) (χML ρml) σ) as (χ1 & ζσ & ζσimm & Hext & Hstorebl & Hdisj & Hstore).
-    1: done.
-    1: done.
-    1: done.
-    destruct (deserialize_ML_values χ1 vv) as (χ2 & ζimm & lvs & Hext2 & Hvs).
-    1: apply Hext.
-
-    assert (ζML ρml ∪ ζσ ∪ ζσimm ##ₘ ζimm) as Hdis1.
-    1: { eapply map_disjoint_dom. eapply disjoint_weaken. 1: eapply Hext2. 2: done.
-         rewrite dom_union_L. eapply union_subseteq. split. 2: by eapply extended_to_dom_subset.
-         rewrite dom_union_L. eapply union_subseteq; split.
-         1: etransitivity; first by eapply elem_of_subseteq. 1: eapply subseteq_dom, Hext.
-         intros γ Hγ. destruct Hstorebl as [_ HR]. apply HR in Hγ. destruct Hγ as (ℓ & ? & HH & _); by eapply elem_of_dom_2. }
-
-    pose (ζML ρml ∪ ζσ ∪ (ζσimm ∪ ζimm)) as ζC.
-
-    destruct (collect_dom_θ_ζ ∅ ζC) as (θdom1 & Hθdom1).
-    destruct (collect_dom_θ_vs θdom1 lvs) as (θdom2 & Hθdom2).
-    destruct (collect_dom_θ_roots θdom2 (rootsML ρml)) as (θdom3 & Hθdom3).
-    destruct (injectivify_map θdom3) as (θC & Hdom & Hinj).
-    destruct (find_repr_lval_vs θC lvs) as (ws & Hws).
-    1: intros γ Hγ; subst θdom3; apply Hθdom3; right; apply Hθdom2; left; done.
+  iSplit.
+  + iDestruct (interp_ML_discarded_locs_pub with "Hσ") as %Hpublocs.
+    iNamed "Hσ". iNamed "SIML".
+    iPureIntro. exists (fun _ => True). eapply mlanguage.head_prim_step. cbn.
+    destruct (ml_to_c_exists vv ρml σ) as (ws & ρc & mem & Hml_to_c); eauto.
     destruct (apply_function_arity F ws) as (HL&_); destruct HL as (ec&Hec).
-    1: rewrite Harity; etransitivity; eapply Forall2_length; done.
-    assert (roots_are_live θC (rootsML ρml)) as Hrootslive.
-    1: { intros a γ H1. subst θdom3. apply Hθdom3. left. by eexists. }
-    destruct (find_repr_roots θC (rootsML ρml) (privmemML ρml)) as (mem & Hrepr); try done.
-
-    eapply (RunFunctionS p F vv ρml σ ζσ (ζσimm ∪ ζimm) lvs ws ec mem χ2 ζC θC (fun _ => True)).
-    1: eapply extended_to_trans; done.
-    1: destruct Hstorebl as [HL HR]; split.
-    1: { intros ℓ  Hℓ. destruct (HL ℓ Hℓ) as (γ & Hγ). exists γ. eapply lookup_weaken; first done. apply Hext2. }
-    1: { intros γ; destruct (HR γ) as [HRL HRH]; split.
-         1: intros H; destruct (HRL H) as (ℓ & Vs & H1 & H2); exists ℓ, Vs; split; try done; eapply lookup_weaken; first done; apply Hext2.
-         intros (ℓ & Vs & H1 & H2). apply HRH. exists ℓ, Vs. split; try done. eapply elem_of_dom_2 in H2. destruct (HL _ H2) as (γ2 & Hγ2).
-         enough (γ2 = γ) as -> by done. eapply Hext2. 2: done. eapply lookup_weaken; first done; eapply Hext2. }
-    1: { intros γ. rewrite dom_union_L. intros [H|H]%elem_of_union; eapply lookup_weaken.
-         1: by eapply Hext. 2: by eapply Hext2. 2: done. 1: apply Hext2. }
-    1: { reflexivity. }
-    1: { rewrite map_union_assoc. apply map_disjoint_union_r_2. 1: done.
-         eapply map_disjoint_dom, disjoint_weaken; first eapply map_disjoint_dom, Hdis1; try done.
-         erewrite ! dom_union_L; set_solver. }
-    1: { intros ℓ vs γ b H1 H2 H3. unfold ζC in *. rewrite ! map_union_assoc. rewrite ! map_union_assoc in H3.
-         apply lookup_union_Some_inv_l in H3.
-         2: apply not_elem_of_dom; intros Hc; apply Hext2 in Hc; congruence.
-         eapply is_heap_elt_weaken. 1: eapply Hstore; try done.
-         2: apply Hext2.
-         + destruct Hstorebl as [HL HR]; destruct (HL ℓ) as [v Hv]; first by eapply elem_of_dom_2.
-           rewrite <- Hv; f_equal; eapply Hext2; try done; eapply lookup_weaken, Hext2; try done.
-         + eapply map_union_subseteq_l. }
-    1: { eapply Forall2_impl; first done. intros ? ? H; eapply is_val_mono; last done; first done.
-         unfold ζC. rewrite ! map_union_assoc. eapply map_union_subseteq_r. done. }
-    1: { split; first done. subst θdom3. intros γ m tg vs γ' _ H2 H3.
-         apply Hθdom3. right. apply Hθdom2. right. apply Hθdom1. right. left. do 4 eexists; done. }
-    1: { done. }
-    1: { done. }
-    1: { done. }
-    1: { done. }
-    1: { done. }
+    { rewrite Harity. eapply ml_to_c_words_length; eauto. }
+    eapply RunFunctionS; eauto.
   + iIntros (X Hstep).
     destruct Hstep as ([] & e1 & Heq & Hstep).
     cbv in Heq; subst e1.
     inversion Hstep.
-    cbv in H1. subst fn vs ρml0 σ0 X0.
-
-    iMod (ghost_var_update_halves with "Hb HAbound") as "(Hnb & Hnb2)".
-    1: iPoseProof (@fractional.fractional _ _ (ghost_var_fractional _ _)) as "[HH _]".
-    iDestruct ("HH" with "[Hnb2]") as "(HAGCbound & HAbound)".
-    1: by assert ((1 / 4 + 1 / 4 = 1 / 2)%Qp) as <- by compute_done.
-    iClear "HH".
-    iMod (ghost_var_update_halves with "HAθ HAGCθ") as "(HAθ & HAGCθ)".
-    iMod (lstore_own_insert_many with "HAζrest") as "(HAζrest & Hζnewimm)".
-    1: apply map_disjoint_union_r in H7 as [H71 H72]; apply H72.
-    iMod (lloc_own_mono with "HAχ") as "HAχ"; first done.
-    assert (ζσ ##ₘ ζnewimm) as Hdisj2 by by eapply is_store_blocks_is_private_blocks_disjoint.
-    apply map_disjoint_union_r in H7 as [H71 H72].
-    assert (ζC = ζσ ∪ (ζML ρml ∪ ζnewimm)) as H6B.
-    1: { rewrite map_union_assoc. rewrite (map_union_comm ζσ); first done. by symmetry. }
-    iPoseProof (block_sim_arr_of_ghost_state _ _ _ _ _ vv lvs with "HAχ HAζrest [] [] [] [] []") as "#Hsim".
-    1-5: iPureIntro. 5: exact H9. 1-3:done. 1: by apply map_disjoint_union_r.
-    iMod (set_to_some with "HAσCv Hrootspto") as "(HAσCv & Hrootspto)"; first done.
-
-    do 3 iModIntro.
-    do 2 iExists _.
-    iSplitR; first (iPureIntro; exact H16).
-
-    iSpecialize ("Hwp" $! θC lvs ws ec).
-    iSplitR "Hnb Hwp HAGCθ HAGCbound HArootss HArootsm Hrootspto".
-    * unfold wrap_state_interp, C_state_interp; cbn.
-      iSplitL "HAσCv HAnCv"; first (iExists nCv; iFrame).
-      iExists ζC, ζσ, (ζML ρml ∪ ζnewimm), χC, σ.
-      iFrame.
-      iSplitL "HvML"; first by iExists _.
-      rewrite pub_locs_in_lstore_insert_priv_store; last done.
-      erewrite pub_locs_in_lstore_mono at 1; last apply H3; last done.
-      iFrame "HAχNone".
-      iPureIntro. split_and!.
-      1: reflexivity.
-      1: done.
-      1: apply map_disjoint_union_r; done.
-      1: done.
-      1: { rewrite dom_union_L. intros γ [H|H]%elem_of_union.
-           - eapply elem_of_weaken; first by eapply Hother_blocks.
-             eapply subseteq_dom, H3.
-           - by eapply elem_of_dom_2, H5. }
-      1: done.
-      1: { split; first done.
-           split; first apply H3.
-           intros γ v1 v2 H1 H2. rewrite H1 in H2. injection H2; intros ->. econstructor. }
-      1: apply H3.
-      1: done.
-    * iApply (wp_simulates with "Hnb").
-      iApply ("Hwp" with "[-] [] [] Hsim"); try done.
-      unfold GC; cbn.
-      iExists (dom (rootsML ρml)), (rootsML ρml).
-      iFrame. done.
+    cbv [fill Wrap.fill wrap_lang] in *. simplify_eq.
+    iMod (wrap_interp_ml_to_c with "Hσ [$]") as "(Hσ & Hnb & HGC & (%lvs & #Hblk & %))";
+      first done.
+    do 3 iModIntro. do 2 iExists _. iSplit; first by iPureIntro. iFrame "Hσ".
+    iApply (wp_simulates with "Hnb").
+    iApply ("Hwp" with "HGC [%] [%] [$]"); eauto.
 Qed.
 
 End Simulation.
-
-
-
